Did some more work on heap conversion

Heap.thy
@@ -10,25 +10,28 @@ primrec ptrSize :: "ptr \<Rightarrow> nat" where
 fun ptr_less :: "ptr \<Rightarrow> ptr \<Rightarrow> bool" where
   "ptr_less x y = (ptrSize x > ptrSize y)"
 
-datatype 'a heap = H "ptr \<Rightarrow> 'a" nat
+datatype 'a heap = H "nat \<Rightarrow> 'a" nat
 
 definition hempty :: "'a heap" where
   "hempty = H (\<lambda>x. undefined) 0"
  
 primrec halloc :: "'a heap \<Rightarrow> 'a \<Rightarrow> 'a heap \<times> ptr" where
-  "halloc (H h hp) a = (H (h(P hp := a)) (Suc hp), P hp)"
+  "halloc (H h hp) a = (H (h(hp := a)) (Suc hp), P hp)"
 
-primrec hlookup :: "'a heap \<Rightarrow> ptr \<Rightarrow> 'a" where
-  "hlookup (H h hp) x = h x"
+fun hlookup :: "'a heap \<Rightarrow> ptr \<Rightarrow> 'a" where
+  "hlookup (H h hp) (P x) = h x"
 
 fun hcontains :: "'a heap \<Rightarrow> ptr \<Rightarrow> bool" where
   "hcontains (H h hp) (P x) = (x < hp)"
 
-primrec heap_all :: "('a \<Rightarrow> bool) \<Rightarrow> 'a heap \<Rightarrow> bool" where
-  "heap_all p (H h hp) = (\<forall>x < hp. p (h (P x)))"
+primrec heap_all :: "(ptr \<Rightarrow> 'a \<Rightarrow> bool) \<Rightarrow> 'a heap \<Rightarrow> bool" where
+  "heap_all p (H h hp) = (\<forall>x < hp. p (P x) (h x))"
+
+primrec hmap :: "('a \<Rightarrow> 'b) \<Rightarrow> 'a heap \<Rightarrow> 'b heap" where
+  "hmap f (H h hp) = H (f \<circ> h) hp"
 
 lemma [simp]: "halloc h a = (h', x) \<Longrightarrow> hlookup h' y = (if x = y then a else hlookup h y) "
-  by (induction h) auto
+  by (induction h y rule: hlookup.induct) (auto split: if_splits)
 
 lemma [simp]: "hcontains h x \<Longrightarrow> halloc h a = (h', y) \<Longrightarrow> hcontains h' x"
   by (induction h x rule: hcontains.induct) auto
@@ -36,16 +39,25 @@ lemma [simp]: "hcontains h x \<Longrightarrow> halloc h a = (h', y) \<Longrighta
 lemma [simp]: "halloc h a = (h', x) \<Longrightarrow> hcontains h' x"
   by (induction h x rule: hcontains.induct) auto
 
-lemma heap_lookup_all: "hlookup h x = a \<Longrightarrow> heap_all p h \<Longrightarrow> hcontains h x \<Longrightarrow> p a"
+lemma heap_lookup_all: "hlookup h x = a \<Longrightarrow> heap_all p h \<Longrightarrow> hcontains h x \<Longrightarrow> p x a"
   by (induction h x rule: hcontains.induct) auto
 
-lemma [elim]: "heap_all p h \<Longrightarrow> halloc h a = (h', x) \<Longrightarrow> p a \<Longrightarrow> heap_all p h'"
+lemma [elim]: "heap_all p h \<Longrightarrow> halloc h a = (h', x) \<Longrightarrow> p x a \<Longrightarrow> heap_all p h'"
   by (induction h) auto
 
-lemma [elim]: "(\<And>x. p x \<Longrightarrow> q x) \<Longrightarrow> heap_all p h \<Longrightarrow> heap_all q h"
+lemma [elim]: "(\<And>x y. p x y \<Longrightarrow> q x y) \<Longrightarrow> heap_all p h \<Longrightarrow> heap_all q h"
   by (induction h) simp_all
 
 lemma [simp]: "heap_all f hempty"
   by (simp add: hempty_def)
+
+lemma [simp]: "halloc h a = (h', x) \<Longrightarrow> hcontains h y \<Longrightarrow> ptrSize y < ptrSize x"
+  by (induction h y rule: hcontains.induct) auto
+
+lemma [simp]: "halloc h a = (h', v) \<Longrightarrow> hcontains h x \<Longrightarrow> v \<noteq> x"
+  by (induction h x rule: hcontains.induct) auto
+
+lemma [simp]: "halloc h a = (h', v) \<Longrightarrow> halloc (hmap f h) (f a) = (hmap f h', v)"
+  by (induction h) auto+
 
 end
