HeapConversion.thy
@@ -2,11 +2,18 @@ theory HeapConversion
   imports HeapMemory
 begin
 
+primrec stack_below :: "ptr \<Rightarrow> ptr list \<Rightarrow> bool" where
+  "stack_below x [] = True"
+| "stack_below x (v # vs) = (ptr_less x v \<and> stack_below x vs)"
+
+lemma [simp]: "stack_below x ys \<Longrightarrow> y \<in> set ys \<Longrightarrow> ptrSize y < ptrSize x"
+  by (induction ys) auto
+
 function unheap_closure :: "hclosure heap \<Rightarrow> ptr \<Rightarrow> bclosure" where
-  [simp del]: "unheap_closure h x = (case hlookup h x of 
+  "unheap_closure h x = (case hlookup h x of 
       HConst k \<Rightarrow> BConst k
     | HLam env pc \<Rightarrow> 
-        BLam (if \<forall>y \<in> set env. ptr_less x y then map (unheap_closure h) env else undefined) pc)"
+        BLam (if stack_below x env then map (unheap_closure h) env else undefined) pc)"
   by pat_completeness auto
 termination by (relation "measure (ptrSize \<circ> snd)") simp_all
 
@@ -14,62 +21,97 @@ primrec unheap :: "heap_state \<Rightarrow> byte_code_state" where
   "unheap (HS h vs envs pcs cd) = 
     BS (map (unheap_closure h) vs) (map (map (unheap_closure h)) envs) pcs cd"
 
-primrec bounded_closure :: "hclosure heap \<Rightarrow> hclosure \<Rightarrow> bool" where
-  "bounded_closure h (HConst k) = True"
-| "bounded_closure h (HLam env pc) = (\<forall>x \<in> set env. hcontains h x)"
+primrec stack_contains :: "hclosure heap \<Rightarrow> ptr list \<Rightarrow> bool" where
+  "stack_contains h [] = True"
+| "stack_contains h (v # vs) = (hcontains h v \<and> stack_contains h vs)"
+
+primrec env_contains :: "hclosure heap \<Rightarrow> ptr list list \<Rightarrow> bool" where
+  "env_contains h [] = True"
+| "env_contains h (v # vs) = (stack_contains h v \<and> env_contains h vs)"
+
+primrec bounded_closure :: "hclosure heap \<Rightarrow> ptr \<Rightarrow> hclosure \<Rightarrow> bool" where
+  "bounded_closure h x (HConst k) = True"
+| "bounded_closure h x (HLam env pc) = (stack_contains h env \<and> stack_below x env)"
 
 primrec heap_structured :: "heap_state \<Rightarrow> bool" where
   "heap_structured (HS h vs envs pcs cd) = (heap_all (bounded_closure h) h \<and>
-    (\<forall>v \<in> set vs. hcontains h v) \<and> (\<forall>env \<in> set envs. \<forall>x \<in> set env. hcontains h x))"
+    stack_contains h vs \<and> env_contains h envs)"
 
-lemma [simp]: "halloc h a = (h', x) \<Longrightarrow> bounded_closure h c \<Longrightarrow> bounded_closure h' c"
-  by (induction c) auto
+lemma [simp]: "halloc h a = (h', x) \<Longrightarrow> stack_contains h vs \<Longrightarrow> stack_contains h' vs"
+  by (induction vs) auto
 
-lemma [simp]: "heap_all (bounded_closure h) h \<Longrightarrow> halloc h c = (h', v) \<Longrightarrow> bounded_closure h c \<Longrightarrow> 
+lemma [simp]: "halloc h a = (h', x) \<Longrightarrow> env_contains h vs \<Longrightarrow> env_contains h' vs"
+  by (induction vs) simp_all
+
+lemma [simp]: "halloc h a = (h', x) \<Longrightarrow> bounded_closure h y c \<Longrightarrow> bounded_closure h' y c"
+  by (induction c) simp_all
+
+lemma [simp]: "lookup vs x = Some v \<Longrightarrow> stack_contains h vs \<Longrightarrow> hcontains h v"
+  by (induction vs x rule: lookup.induct) simp_all
+
+lemma [simp]: "heap_all (bounded_closure h) h \<Longrightarrow> halloc h c = (h', v) \<Longrightarrow> bounded_closure h v c \<Longrightarrow> 
     heap_all (bounded_closure h') h'"
 proof -
-  assume A: "halloc h c = (h', v)" and "heap_all (bounded_closure h) h" and "bounded_closure h c"
+  assume A: "halloc h c = (h', v)" and "heap_all (bounded_closure h) h" and "bounded_closure h v c"
   hence "heap_all (bounded_closure h) h'" by auto
-  moreover from A have "\<And>c. bounded_closure h c \<Longrightarrow> bounded_closure h' c" by simp
+  moreover from A have "\<And>x c. bounded_closure h x c \<Longrightarrow> bounded_closure h' x c" by simp
   ultimately show ?thesis by auto
 qed
+
+lemma [simp]: "halloc h (HConst k) = (h', v) \<Longrightarrow> unheap_closure h' v = BConst k"
+  by simp
+
+lemma [simp]: "halloc h c = (h', v) \<Longrightarrow> stack_contains h env \<Longrightarrow> stack_below v env"
+  by (induction env) simp_all
+
+lemma [elim]: "stack_contains h env \<Longrightarrow> x \<in> set env \<Longrightarrow> hcontains h x"
+  by (induction env) auto
+
+lemma [simp]: "halloc h c = (h', v) \<Longrightarrow> hcontains h x \<Longrightarrow> heap_all (bounded_closure h) h \<Longrightarrow> 
+  unheap_closure h' x = unheap_closure h x"
+proof (induction h x rule: unheap_closure.induct)
+  case (1 h x)
+  thus ?case
+  proof (cases "hlookup h x")
+    case (HLam env p)
+    with 1 show ?thesis
+    proof (cases "stack_below x env")
+      case True
+      from HLam 1 have "stack_contains h env" by (metis heap_lookup_all bounded_closure.simps(2))
+      hence S: "\<And>y. y \<in> set env \<Longrightarrow> hcontains h y" by auto
+      from 1 HLam True have "\<And>y. y \<in> set env \<Longrightarrow> hcontains h y \<Longrightarrow> 
+        unheap_closure h' y = unheap_closure h y" by simp
+      with S 1(2, 3) HLam True show ?thesis by simp
+    qed simp_all
+  qed simp_all
+qed
+
+lemma [simp]: "halloc h c = (h', v) \<Longrightarrow> stack_contains h env \<Longrightarrow> heap_all (bounded_closure h) h \<Longrightarrow>
+    map (unheap_closure h') env = map (unheap_closure h) env"
+  by (induction env) (simp_all del: unheap_closure.simps)
+
+lemma [simp]: "halloc h c = (h', v) \<Longrightarrow> env_contains h env \<Longrightarrow> heap_all (bounded_closure h) h \<Longrightarrow>
+    map (map (unheap_closure h')) env = map (map (unheap_closure h)) env"
+  by (induction env) (simp_all del: unheap_closure.simps)
+
+lemma [simp]: "halloc h (HLam env p) = (h', v) \<Longrightarrow> stack_contains h env \<Longrightarrow> 
+    heap_all (bounded_closure h) h \<Longrightarrow> unheap_closure h' v = BLam (map (unheap_closure h) env) p"
+  by simp
+
+lemma [simp]: "hlookup h v = HLam env pc \<Longrightarrow> heap_all (bounded_closure h) h \<Longrightarrow> hcontains h v \<Longrightarrow>
+    stack_below v env"
+  by (metis heap_lookup_all bounded_closure.simps(2))
 
 lemma [simp]: "\<Sigma>\<^sub>h \<leadsto>\<^sub>h \<Sigma>\<^sub>h' \<Longrightarrow> heap_structured \<Sigma>\<^sub>h \<Longrightarrow> heap_structured \<Sigma>\<^sub>h'"
 proof (induction \<Sigma>\<^sub>h \<Sigma>\<^sub>h' rule: evalh.induct)
   case (evh_apply cd pc h v2 env pc' v1 vs envs pcs)
   hence "hlookup h v2 = HLam env pc' \<and> heap_all (bounded_closure h) h \<and> hcontains h v2" by simp
-  hence "bounded_closure h (HLam env pc')" by (metis heap_lookup_all)
+  hence "bounded_closure h v2 (HLam env pc')" by (metis heap_lookup_all)
   with evh_apply show ?case by simp
 qed fastforce+
 
 theorem correcth [simp]: "\<Sigma>\<^sub>h \<leadsto>\<^sub>h \<Sigma>\<^sub>h' \<Longrightarrow> heap_structured \<Sigma>\<^sub>h \<Longrightarrow> unheap \<Sigma>\<^sub>h \<leadsto>\<^sub>b unheap \<Sigma>\<^sub>h'"
-proof (induction \<Sigma>\<^sub>h \<Sigma>\<^sub>h' rule: evalh.induct)
-  case (evh_pushcon cd pc k h h' v vs env envs pcs)
-  from evh_pushcon have "cd ! pc = BPushCon k" by simp
-  from evh_pushcon have "halloc h (HConst k) = (h', v)" by simp
-
-  from evh_pushcon have "heap_all (bounded_closure h) h" by simp
-  from evh_pushcon have "\<forall>v\<in>set vs. hcontains h v" by simp
-  from evh_pushcon have "\<forall>x\<in>set env. hcontains h x" by simp
-  from evh_pushcon have "\<forall>env\<in>set envs. \<forall>x\<in>set env. hcontains h x" by simp
-
-
-  from evh_pushcon have 
-       "BS (unheap_closure h' v # map (unheap_closure h') vs) (map (map (unheap_closure h')) envs) (pc # pcs) cd = 
-    BS (BConst k # (map (unheap_closure h) vs)) (map (map (unheap_closure h)) envs) (pc # pcs) cd" 
-    by simp
-
-
-  have "BS (map (unheap_closure h) vs) (map (unheap_closure h) env # map (map (unheap_closure h)) envs) (Suc pc # pcs) cd \<leadsto>\<^sub>b
-    BS (unheap_closure h' v # map (unheap_closure h') vs) (map (map (unheap_closure h')) envs) (pc # pcs) cd" by simp
-  then show ?case by simp
-next
-  case (evh_pushlam cd pc pc' h env h' v vs envs pcs)
-  then show ?case by simp
-next
-  case (evh_apply cd pc h v2 env pc' v1 vs envs pcs)
-  then show ?case by simp
-qed simp_all
+  by (induction \<Sigma>\<^sub>h \<Sigma>\<^sub>h' rule: evalh.induct) simp_all
 
 lemma unheap_backwards [simp]: "BS vs envs pcs cd = unheap \<Sigma>\<^sub>h \<Longrightarrow> \<exists>h vs' envs'. 
   \<Sigma>\<^sub>h = HS h vs' envs' pcs cd \<and> vs = map (unheap_closure h) vs' \<and> 
@@ -80,22 +122,40 @@ theorem completeh [simp]: "unheap \<Sigma>\<^sub>h \<leadsto>\<^sub>b \<Sigma>\<
   \<exists>\<Sigma>\<^sub>h'. \<Sigma>\<^sub>h \<leadsto>\<^sub>h \<Sigma>\<^sub>h' \<and> \<Sigma>\<^sub>b' = unheap \<Sigma>\<^sub>h'"
 proof (induction "unheap \<Sigma>\<^sub>h" \<Sigma>\<^sub>b' rule: evalb.induct)
   case (evb_lookup cd pc x env v vs envs pcs)
-  thus ?case by simp
+  then obtain h vs' envs'' where S: "\<Sigma>\<^sub>h = HS h vs' envs'' (Suc pc # pcs) cd \<and> 
+    vs = map (unheap_closure h) vs' \<and> env # envs = map (map (unheap_closure h)) envs''" by fastforce
+  then obtain env' envs' where E: "envs'' = env' # envs' \<and> env = map (unheap_closure h) env' \<and> 
+    envs = map (map (unheap_closure h)) envs'" by fastforce
+
+
+
+  from evb_lookup have "cd ! pc = BLookup x" by simp
+  from evb_lookup have "lookup env x = Some v" by simp
+  from evb_lookup have "heap_structured \<Sigma>\<^sub>h" by simp
+
+
+  have "cd ! pc = BLookup x \<Longrightarrow> lookup env' x = Some vv \<Longrightarrow> 
+    HS h vs' (env' # envs') (Suc pc # pcs) cd \<leadsto>\<^sub>h HS h (vv # vs') envs' (pc # pcs) cd" by simp
+
+  have X: "HS h vs' (env' # envs') (Suc pc # pcs) cd \<leadsto>\<^sub>h \<Sigma>\<^sub>h'" by simp
+  have "BS (v # map (unheap_closure h) vs') (map (map (unheap_closure h)) envs') (pc # pcs) cd = unheap \<Sigma>\<^sub>h'" 
+      by simp
+  with S E X show ?case by fastforce
 next
   case (evb_pushcon cd pc k vs env envs pcs)
-  then show ?case by simp
+  thus ?case by simp
 next
   case (evb_pushlam cd pc pc' vs env envs pcs)
-  then show ?case by simp
+  thus ?case by simp
 next
   case (evb_enter cd pc vs env envs pcs)
-  then show ?case by simp
+  thus ?case by simp
 next
   case (evb_apply cd pc v env pc' vs envs pcs)
-  then show ?case by simp
+  thus ?case by simp
 next
   case (evb_return cd pc vs envs pcs)
-  then show ?case by simp
+  thus ?case by simp
 qed
 
 lemma [simp]: "iter (\<leadsto>\<^sub>b) (unheap \<Sigma>\<^sub>h) \<Sigma>\<^sub>b' \<Longrightarrow> heap_structured \<Sigma>\<^sub>h \<Longrightarrow> 
